finish proof about compiler output and factor out remaining admits
WIP, working on compiler proof

compiler proof statement

wip separating proof

WIP

wip, changed ext_spec in field25519 to be parameterized

wip

finish proof about compiler output and factor out remaining admits

src/Bedrock/End2End/X25519/MontgomeryLadder.v
@@ -2,11 +2,14 @@ Require Import Coq.Strings.String.
 Require Import Coq.Lists.List.
 Require Import Coq.ZArith.ZArith.
 Require Import Crypto.Spec.Curve25519.
+Require Import bedrock2.Map.Separation.
 Require Import bedrock2.Syntax.
 Require Import compiler.Pipeline.
 Require Import compiler.MMIO.
+Require Import coqutil.Word.Bitwidth32.
 Require Import Crypto.Arithmetic.PrimeFieldTheorems.
 Require Import Crypto.Bedrock.End2End.X25519.Field25519.
+Require Import Crypto.Bedrock.Field.Interface.Compilation2.
 Require Import Crypto.Bedrock.Field.Synthesis.New.UnsaturatedSolinas.
 Require Import Crypto.Bedrock.Group.AdditionChains.
 Require Import Crypto.Bedrock.Group.ScalarMult.LadderStep.
@@ -15,17 +18,24 @@ Require Import Crypto.Bedrock.Group.ScalarMult.MontgomeryLadder.
 Local Open Scope string_scope.
 Import ListNotations.
 
-Definition ladderstep : func :=
-  Eval vm_compute in
-    (ladderstep_body
-      (field_parameters:=field_parameters)
-      (field_representaton:=field_representation n s c)).
 
-Definition montladder : func :=
-  Eval vm_compute in
-    (montladder_body (Z.to_nat (Z.log2_up Curve25519.l))
-      (field_parameters:=field_parameters)
-      (field_representaton:=field_representation n s c)).
+Derive ladderstep SuchThat
+       (ladderstep = ladderstep_body
+                       (BW:=BW32)
+                       (field_parameters:=field_parameters)
+                       (field_representaton:=field_representation n s c))
+       As ladderstep_defn.
+Proof. vm_compute. subst; exact eq_refl. Qed.
+
+Derive montladder SuchThat
+       (montladder
+        = montladder_body
+            (BW:=BW32)
+            (Z.to_nat (Z.log2_up Curve25519.l))
+            (field_parameters:=field_parameters)
+            (field_representaton:=field_representation n s c))
+       As montladder_defn.
+Proof. vm_compute. subst; exact eq_refl. Qed.
 
 Definition funcs : list func :=
   [
@@ -48,8 +58,11 @@ Require Import bedrock2.ToCString.
 Compute c_module funcs.
 *)
 
-Definition compiler_test_out := Eval vm_compute in
-  compile (compile_ext_call (funname_env:=SortedListString.map)) (map.of_list funcs).
-Compute
-  match compiler_test_out with
-  Success ((x, z), y) => Success (length x, z) | Failure e => Failure e end.
+Derive montladder_compiler_result SuchThat
+       (compile
+         (compile_ext_call (funname_env:=SortedListString.map))
+         (map.of_list funcs) = Success montladder_compiler_result)
+       As montladder_compiler_result_ok.
+Proof.
+  vm_compute. apply f_equal. subst; exact eq_refl.
+Qed.
